refreshability_tac

thys/MRBNF_FP.thy
@@ -333,4 +333,46 @@ ML_file \<open>../Tools/mrbnf_fp.ML\<close>
 ML_file \<open>../Tools/mrbnf_recursor_tactics.ML\<close>
 ML_file \<open>../Tools/mrbnf_recursor.ML\<close>
 
+ML \<open>
+local
+  open BNF_Util
+in
+
+fun refreshability_tac B Tsupp G_thm small_thms instss simp_thms intro_thms ctxt =
+  let
+    val fresh = infer_instantiate' ctxt
+      [SOME (Thm.cterm_of ctxt B), SOME (Thm.cterm_of ctxt Tsupp),
+       SOME (Thm.cterm_of ctxt (HOLogic.mk_binop \<^const_name>\<open>minus\<close> (Tsupp, B)))]
+      @{thm eextend_fresh};
+    val small_ctxt = ctxt addsimps small_thms;
+    fun case_tac NONE _ prems ctxt = SOLVE (auto_tac (ctxt addsimps prems))
+      | case_tac (SOME insts) params prems ctxt =
+        let
+          val f = hd params |> snd |> Thm.term_of;
+          val ex_f = infer_instantiate' ctxt [NONE, SOME (Thm.cterm_of ctxt f)] exI;
+          val args = tl params |> map (snd #> Thm.term_of);
+          val xs = @{map 2} (fn i => fn a => Thm.cterm_of ctxt (i $ f $ a)) insts args;
+          val id_onI = nth prems 3 RS @{thm id_on_antimono};
+        in
+          HEADGOAL (EVERY' (map (fn x => rtac ctxt (infer_instantiate' ctxt [NONE, SOME x] exI)) xs)) THEN
+          SOLVE (HEADGOAL (SELECT_GOAL (mk_auto_tac (ctxt
+            addsimps (simp_thms @ prems)
+            addSIs (ex_f :: id_onI :: intro_thms)) 0 4) THEN_ALL_NEW
+            SELECT_GOAL (print_tac ctxt "auto failed")))
+        end;
+  in
+    HEADGOAL (rtac ctxt (fresh RS exE) THEN'
+      rtac ctxt (G_thm RSN (2, cut_rl)) THEN' SELECT_GOAL (auto_tac small_ctxt) THEN'
+      REPEAT_DETERM_N 4 o simp_tac small_ctxt THEN'
+      REPEAT_DETERM o etac ctxt conjE THEN'
+      EVERY' [rtac ctxt exI, rtac ctxt conjI, assume_tac ctxt] THEN'
+      rtac ctxt (G_thm RSN (2, cut_rl)) THEN'
+      REPEAT_ALL_NEW (eresolve_tac ctxt @{thms exE conjE disj_forward}) THEN'
+      EVERY' (map (fn insts => Subgoal.FOCUS (fn focus =>
+        case_tac insts (#params focus) (#prems focus) (#context focus)) ctxt) instss))
+  end;
+
+end;
+\<close>
+
 end
