thys/Untyped_Lambda_Calculus/LC_Beta_depth.thy
@@ -18,7 +18,49 @@ inductive stepD :: "nat \<Rightarrow> trm \<Rightarrow> trm \<Rightarrow> bool" 
 | AppL: "stepD d e1 e1' \<Longrightarrow> stepD (Suc d) (App e1 e2) (App e1' e2)"
 | AppR: "stepD d e2 e2' \<Longrightarrow> stepD (Suc d) (App e1 e2) (App e1 e2')"
 | Xi: "stepD d e e' \<Longrightarrow> stepD d (Lam x e) (Lam x e')"
+ML \<open>
+local
+  open BNF_Util
+in
 
+fun refreshability_tac B Tsupp G_thm small_thms instss simp_thms intro_thms ctxt =
+  let
+    val fresh = infer_instantiate' ctxt
+      [SOME (Thm.cterm_of ctxt B), SOME (Thm.cterm_of ctxt Tsupp),
+       SOME (Thm.cterm_of ctxt (HOLogic.mk_binop \<^const_name>\<open>minus\<close> (Tsupp, B)))]
+      @{thm eextend_fresh};
+    val small_ctxt = ctxt addsimps small_thms;
+    fun case_tac NONE _ prems ctxt = SOLVE (auto_tac (ctxt addsimps prems))
+      | case_tac (SOME insts) params prems ctxt =
+        let
+          val f = hd params |> snd |> Thm.term_of;
+          val ex_f = infer_instantiate' ctxt [NONE, SOME (Thm.cterm_of ctxt f)] exI;
+          val args = tl params |> map (snd #> Thm.term_of);
+          val xs = @{map 2} (fn i => fn a => Thm.cterm_of ctxt (i $ f $ a)) insts args;
+          val id_onI = nth prems 3 RS @{thm id_on_antimono};
+        in
+          HEADGOAL (EVERY' (map (fn x => rtac ctxt (infer_instantiate' ctxt [NONE, SOME x] exI)) xs)) THEN
+print_tac ctxt "foo" THEN
+          SOLVE (HEADGOAL (SELECT_GOAL (mk_auto_tac (ctxt
+            addsimps (simp_thms @ prems)
+            addSIs (ex_f :: id_onI :: intro_thms)) 0 4) THEN_ALL_NEW
+            SELECT_GOAL (print_tac ctxt "auto failed")))
+        end;
+  in
+    HEADGOAL (rtac ctxt (fresh RS exE) THEN'
+      rtac ctxt (G_thm RSN (2, cut_rl)) THEN' SELECT_GOAL (auto_tac small_ctxt) THEN'
+      REPEAT_DETERM_N 4 o simp_tac small_ctxt THEN'
+      REPEAT_DETERM o etac ctxt conjE THEN'
+      EVERY' [rtac ctxt exI, rtac ctxt conjI, assume_tac ctxt] THEN'
+K (print_tac ctxt "bar") THEN'
+      rtac ctxt (G_thm RSN (2, cut_rl)) THEN'
+      REPEAT_ALL_NEW (eresolve_tac ctxt @{thms exE conjE disj_forward}) THEN'
+      EVERY' (map (fn insts => Subgoal.FOCUS (fn focus =>
+        case_tac insts (#params focus) (#prems focus) (#context focus)) ctxt) instss))
+  end;
+
+end;
+\<close>
 binder_inductive stepD where
   Beta binds x
 | Xi binds x
@@ -30,12 +72,22 @@ for perms: "\<lambda>_. id" rrename rrename and supps: "\<lambda>_. {}" FFVars_t
       (auto simp: isPerm_def term.rrename_comps rrename_tvsubst_comp
         | ((rule exI[of _ "\<sigma> _"] exI)+, (rule conjI)?, rule refl)
         | ((rule exI[of _ "\<sigma> _"])+; auto))+
-  subgoal premises prems for R B x1 x2 x3
-    using fresh[of x2 x3] prems(2-)
-    unfolding ex_push_inwards conj_disj_distribL ex_disj_distrib
-    apply (elim disj_forward exE; simp)
-     apply (metis Lam_eq_tvsubst Lam_refresh singletonD)
-    by blast
+  subgoal premises prems for R B d t1 t2
+    apply (tactic \<open>refreshability_tac @{term B} @{term "Tsupp d t1 t2"}
+      @{thm prems(3)} @{thms emp_bound singl_bound term.Un_bound term.card_of_FFVars_bounds infinite}
+      [SOME [@{term "(\<lambda>f x. f x) :: (var \<Rightarrow> var) \<Rightarrow> var \<Rightarrow> var"},
+             @{term "rrename :: (var \<Rightarrow> var) \<Rightarrow> trm \<Rightarrow> trm"},
+             @{term "(\<lambda>f e. e) :: (var \<Rightarrow> var) \<Rightarrow> trm \<Rightarrow> trm"}],
+       NONE,
+       NONE,
+       SOME [@{term "(\<lambda>f d. id d) :: (var \<Rightarrow> var) \<Rightarrow> nat \<Rightarrow> nat"},
+             @{term "rrename :: (var \<Rightarrow> var) \<Rightarrow> trm \<Rightarrow> trm"},
+             @{term "rrename :: (var \<Rightarrow> var) \<Rightarrow> trm \<Rightarrow> trm"},
+             @{term "(\<lambda>f x. f x) :: (var \<Rightarrow> var) \<Rightarrow> var \<Rightarrow> var"}]]
+      @{thms Lam_inject}
+      @{thms prems(2) Lam_eq_tvsubst term.rrename_cong_ids[symmetric]}
+      @{context}\<close>)
+    done
   done
 
 thm stepD.strong_induct
